Examples/LambdaCalcKit.lean
@@ -16,11 +16,11 @@ namespace LeanSubst.Examples.LambdaCalc
   | su t => t
 
   @[simp, grind =]
-  theorem Term.from_action_id {n} : from_action (+0.act n) = var n := by
+  theorem Term.from_action_id {n} : from_action (+0σ.act n) = var n := by
     simp [from_action, Subst.id]
 
   @[simp, grind =]
-  theorem Term.from_action_succ {n} : from_action (+1.act n) = var (n + 1) := by
+  theorem Term.from_action_succ {n} : from_action (+1σ.act n) = var (n + 1) := by
     simp [from_action, Subst.succ]
 
   @[simp, grind =]
@@ -105,7 +105,7 @@ namespace LeanSubst.Examples.LambdaCalc
     simp +instances [SubstMap.smap]
 
   @[simp]
-  theorem Term.from_action_compose {x} {σ τ : Subst Term}
+  theorem Term.from_action_compose {x : Nat} {σ τ : Subst Term}
     : (from_action (σ.act x))[τ] = from_action ((σ ∘ τ).act x)
   := by
     simp [Term.from_action, Subst.compose]
@@ -113,7 +113,7 @@ namespace LeanSubst.Examples.LambdaCalc
     cases z <;> simp [Term.from_action]
 
   @[simp]
-  theorem Term.from_action_compose_ren {x} {σ : Subst Term} {r : Ren Term}
+  theorem Term.from_action_compose_ren {x : Nat} {σ : Subst Term} {r : Ren Term}
     : (from_action (σ.act x))⟨r⟩ = from_action ((σ ∘ r).act x)
   := by
     simp [Term.from_action]
@@ -129,7 +129,7 @@ namespace LeanSubst.Examples.LambdaCalc
   instance : SubstMapRenComposeLeft Term Term where
     apply_ren_compose_left := by subst_solve_compose
 
-  instance : SubstMapRenComposeRight Term where
+  instance : SubstMapRenComposeRight Term Term where
     apply_ren_compose_right := by subst_solve_compose
 
   instance : SubstMapCompose Term Term where
